**Change of basis**
Consider the basic $\{ \vec{b}_{1},\vec{b}_{2} \}$ and $\{ \vec{c}_{1}, \vec{c}_{2} \}$ for a vector space $V$
If $\vec{b}_{1}$

---
In general, if $\{ \vec{b}_1, \dots , \vec{b_n} \}$ and $\{ \vec{c}_1, \dots , \vec{c_n} \}$ are two bases, $[\vec{b}_{1}]_{c}$ is a vector in $\mathbb{R}^n$, $[\vec{b}_{2}]_{c} \dots [\vec{b}_{n}]_{c}$

Then any vector $\vec{x}$ with $[x]_{B} \in \mathbb{R}^n$
$[\vec{x}]_{c}$
$$
=[x_{1}\vec{b}_{1}+\dots x_{n}\vec{b}_{n}]_{c}
$$
$$
=x_{1}[\vec{b}_{1}]_{c}+\dots+x_{n}[\vec{b}_{n}]_{c}
$$
$$
=[[\vec{b}_{1}]_{c}+\dots+[\vec{b}_{n}]_{c}][\vec{x}]_{B}
$$

---
eg:
Let
$$
\vec{b}_{1}=\begin{bmatrix}
-9 \\
1
\end{bmatrix}, \vec{b}_{2} = \begin{bmatrix}
-5 \\
-1
\end{bmatrix}
, \vec{c}_{1}=\begin{bmatrix}
1 \\
-4
\end{bmatrix}, \vec{c}_{2} = \begin{bmatrix}
3 \\
-5
\end{bmatrix}
$$ 
Find the change of coordinates matrix from $B$ to $C$
Solution:
$\vec{b}_{1}=x_{1}\vec{c}_{1}+x_{2}\vec{c}_{2}$
$\vec{b}_{2}=y\vec{c}_{1}+y_{2}\vec{c}_{2}$
Then: $P = \begin{bmatrix}x_{1}  & y_{1} \\ x_{2} & y_{2}\end{bmatrix}$

Augmented:
$$
\begin{bmatrix}
\vec{c}_{1} & \vec{c}_{2}
\end{bmatrix} \begin{bmatrix}
x_{1} \\
x_{2}
\end{bmatrix}=\vec{b}_{1}=\begin{bmatrix}
-4 \\
1
\end{bmatrix}
$$
$$
\begin{bmatrix}
\vec{c}_{1} & \vec{c}_{2}
\end{bmatrix} \begin{bmatrix}
y_{1} \\
y_{2}
\end{bmatrix}=\vec{b}_{1}=\begin{bmatrix}
-5 \\
-1
\end{bmatrix}
$$
$$
\begin{bmatrix}
\vec{c}_{1} ,\vec{c}_{2} & | & \vec{b}_{1},\vec{b}_{2}
\end{bmatrix} \to [I_{2}|\vec{x},\vec{y}]
$$
$$
\begin{bmatrix}
1 & 3 & | & -4 & -5 \\
-4 & -5 & | & 1 & -1
\end{bmatrix}
\sim \begin{bmatrix}
1 & 0 & | & 6 & 4 \\
0 & 1 & | & -5 & -3
\end{bmatrix}
$$
$$
P=\begin{bmatrix}
6 & 4 \\
-5 & -3
\end{bmatrix}
$$

---
Eg.
let:
$$
\vec{b}_{1} = \begin{bmatrix}
1 \\
-3
\end{bmatrix}
,\vec{b}_{2} = \begin{bmatrix}
-2 \\
4
\end{bmatrix}
,\vec{c}_{1} = \begin{bmatrix}
-7 \\
9
\end{bmatrix},
\vec{c}_{2} = \begin{bmatrix}
-5 \\
-7
\end{bmatrix}
$$
**a) find the change of coordinates matrix from c to b**
**b) do the same for b to c**
Solution:
$$
P_{C\to B}\space\space\space [\vec{b}_{1},\vec{b}_{2} | \vec{c}_{1}, \vec{c}_{2}]
$$
$$
\begin{bmatrix}
1 & -2 & | & -7 & -5 \\
-3 & 4 & | & 9 & 7
\end{bmatrix}
$$

$$
\sim \begin{bmatrix}
1 & -2 & | & -7 & -5 \\
0 & -2 & | & -12 & -8
\end{bmatrix}
$$
$$
\sim \begin{bmatrix}
1 & 0 & | & 5 & 3 \\
0 & -2 & | & -12 & -8
\end{bmatrix}
$$
$$
\sim \begin{bmatrix}
1 & 0 & | & 5 & 3 \\
0 & 1 & | & 6 & 4
\end{bmatrix}
$$
And the right side gives us $P_{B\to C}$. We want to find $P_{C\to B}$, which is logically the inverse:
$$
P_{C\to B} = \left( P_{B\to C} \right)^{-1} = \frac{1}{5\cdot{4}-3\cdot {6}}\begin{bmatrix}
4 & 6 \\
3 & 5
\end{bmatrix}
$$
$$
= \frac{1}{2}\begin{bmatrix}
4 & 6 \\
3 & 5
\end{bmatrix}
$$

